Verity/Core/Free/TypedIRLowering.lean
@@ -65,6 +65,11 @@ where
         [ .if_ (lowerTExpr cond) (lowerTStmts thenBranch)
         , .if_ (.call "iszero" [lowerTExpr cond]) (lowerTStmts elseBranch)
         ]
+    | .stop => [.expr (.call "stop" [])]
+    | .returnUint value =>
+        [ .expr (.call "mstore" [.lit 0, lowerTExpr value])
+        , .expr (.call "return" [.lit 0, .lit 32])
+        ]
     | .expr value => [.expr (lowerTExpr value)]
     | .revert _reason => [.expr (.call "revert" [.lit 0, .lit 0])]
 
